HOL/Logic_Thms.thy
@@ -9,32 +9,32 @@ theory Logic_Thms
 imports Auto2_HOL
 begin
 
-text \<open>Trivial contradictions\<close>
+(* Trivial contradictions. *)
 setup \<open>add_resolve_prfstep @{thm HOL.refl}\<close>
 setup \<open>add_forward_prfstep @{thm contra_triv}\<close>
 setup \<open>add_resolve_prfstep @{thm TrueI}\<close>
-lemma FalseD [resolve]: "\<not>False" by simp
+theorem FalseD [resolve]: "\<not>False" by simp
 lemma exists_triv_eq [resolve]: "\<exists>x. x = x" by auto
 
-text \<open>Not\<close>
+(* Not. *)
 setup \<open>add_forward_prfstep_cond @{thm HOL.not_sym} [with_filt (not_type_filter "s" boolT)]\<close>
 
-text \<open>Iff\<close>
+(* Iff. *)
 setup \<open>add_gen_prfstep ("iff_intro1",
   [WithGoal @{term_pat "(?A::bool) = ?B"},
    CreateCase @{term_pat "?A::bool"},
    WithScore 25])\<close>
-lemma iff_goal:
+theorem iff_goal:
   "A \<noteq> B \<Longrightarrow> A \<Longrightarrow> \<not>B" "A \<noteq> B \<Longrightarrow> B \<Longrightarrow> \<not>A"
   "A \<noteq> B \<Longrightarrow> \<not>A \<Longrightarrow> B" "A \<noteq> B \<Longrightarrow> \<not>B \<Longrightarrow> A"
   "(\<not>A) \<noteq> B \<Longrightarrow> A \<Longrightarrow> B" "A \<noteq> (\<not>B) \<Longrightarrow> B \<Longrightarrow> A" by auto
 setup \<open>fold (fn th => add_forward_prfstep_cond th [with_score 1]) @{thms iff_goal}\<close>
 
-text \<open>Quantifiers: normalization\<close>
-lemma exists_split: "(\<exists>x y. P x \<and> Q y) = ((\<exists>x. P x) \<and> (\<exists>y. Q y))" by simp
+(* Quantifiers: normalization *)
+theorem exists_split: "(\<exists>x y. P x \<and> Q y) = ((\<exists>x. P x) \<and> (\<exists>y. Q y))" by simp
 setup \<open>add_backward_prfstep (equiv_backward_th @{thm exists_split})\<close>
 
-text \<open>Case analysis\<close>
+(* Case analysis. *)
 setup \<open>add_gen_prfstep ("case_intro",
   [WithTerm @{term_pat "if ?cond then (?yes::?'a) else ?no"},
    CreateCase @{term_pat "?cond::bool"}])\<close>
@@ -53,21 +53,21 @@ lemma ifb_eval:
 setup \<open>fold (fn th => add_rewrite_rule_cond th [with_score 1])
   ([@{thm HOL.if_P}, @{thm HOL.if_not_P}, @{thm if_eval'}] @ @{thms ifb_eval})\<close>
 
-text \<open>THE and \<exists>!\<close>
+(* THE and \<exists>! *)
 setup \<open>add_forward_prfstep_cond @{thm theI'} [with_term "THE x. ?P x"]\<close>
 setup \<open>add_gen_prfstep ("ex1_case",
   [WithGoal @{term_pat "\<exists>!x. ?P x"}, CreateConcl @{term_pat "\<exists>x. ?P x"}])\<close>
-lemma ex_ex1I' [backward1]: "\<forall>y. P y \<longrightarrow> x = y \<Longrightarrow> P x \<Longrightarrow> \<exists>!x. P x" by auto
-lemma the1_equality': "P a \<Longrightarrow> \<exists>!x. P x \<Longrightarrow> (THE x. P x) = a" by (simp add: the1_equality)
+theorem ex_ex1I' [backward1]: "\<forall>y. P y \<longrightarrow> x = y \<Longrightarrow> P x \<Longrightarrow> \<exists>!x. P x" by auto
+theorem the1_equality': "P a \<Longrightarrow> \<exists>!x. P x \<Longrightarrow> (THE x. P x) = a" by (simp add: the1_equality)
 setup \<open>add_forward_prfstep_cond @{thm the1_equality'} [with_term "THE x. ?P x"]\<close>
 
-text \<open>Hilbert choice\<close>
+(* Hilbert choice. *)
 setup \<open>add_gen_prfstep ("SOME_case_intro",
   [WithTerm @{term_pat "SOME k. ?P k"}, CreateConcl @{term_pat "\<exists>k. ?P k"}])\<close>
 setup \<open>add_forward_prfstep_cond @{thm someI} [with_term "SOME x. ?P x"]\<close>
 setup \<open>add_forward_prfstep_cond @{thm someI_ex} [with_term "SOME x. ?P x"]\<close>
 
-text \<open>Axiom of choice\<close>
+(* Axiom of choice *)
 setup \<open>add_prfstep_custom ("ex_choice",
   [WithGoal @{term_pat "EX f. !x. ?Q f x"}],
   (fn ((id, _), ths) => fn _ => fn _ =>
@@ -79,11 +79,11 @@ setup \<open>add_prfstep_custom ("ex_choice",
     handle THM _ => []))
 \<close>
 
-text \<open>Least operator\<close>
-lemma Least_equality' [backward1]:
+(* Least operator. *)
+theorem Least_equality' [backward1]:
   "P (x::('a::order)) \<Longrightarrow> \<forall>y. P y \<longrightarrow> x \<le> y \<Longrightarrow> Least P = x" by (simp add: Least_equality)
 
-text \<open>Pairs\<close>
+(* Pairs. *)
 lemma pair_inj: "(a,b) = c \<longleftrightarrow> a = fst c \<and> b = snd c" by auto
 setup \<open>Normalizer.add_inj_struct_data @{thm pair_inj}\<close>
 
@@ -93,16 +93,16 @@ setup \<open>add_forward_prfstep (equiv_forward_th @{thm prod.simps(1)})\<close>
 setup \<open>add_rewrite_rule_cond @{thm surjective_pairing} [with_cond "?t \<noteq> (?a, ?b)"]\<close>
 setup \<open>Normalizer.add_rewr_normalizer ("rewr_case", (to_meta_eq @{thm case_prod_beta'}))\<close>
 
-text \<open>Let\<close>
+(* Let. *)
 setup \<open>Normalizer.add_rewr_normalizer ("rewr_let", @{thm Let_def})\<close>
 
-text \<open>Equivalence relations\<close>
+(* Equivalence relations *)  
 setup \<open>add_forward_prfstep @{thm Relation.symD}\<close>
 setup \<open>add_backward_prfstep @{thm Relation.symI}\<close>
 setup \<open>add_forward_prfstep @{thm Relation.transD}\<close>
 setup \<open>add_backward_prfstep @{thm Relation.transI}\<close>
 
-text \<open>Options\<close>
+(* Options *)
 setup \<open>add_resolve_prfstep @{thm option.distinct(1)}\<close>
 setup \<open>add_rewrite_rule @{thm Option.option.sel}\<close>
 setup \<open>add_forward_prfstep @{thm option.collapse}\<close>
