HOL/Pelletier.thy
@@ -1,6 +1,9 @@
 (*
   File: Pelletier.thy
   Author: Bohua Zhan
+
+  Pelletier's problems. From the paper "Seventy-five problems for testing
+  automatic theorem provers" by Francis Jeffry Pelletier.
 *)
 
 section \<open>Pelletier's problems\<close>
@@ -8,11 +11,6 @@ section \<open>Pelletier's problems\<close>
 theory Pelletier
   imports Logic_Thms
 begin
-
-text \<open>
-  Pelletier's problems. From the paper "Seventy-five problems for testing
-  automatic theorem provers" by Francis Jeffry Pelletier.
-\<close>
 
 theorem p1: "(p \<longrightarrow> q) \<longleftrightarrow> (\<not>q \<longrightarrow> \<not>p)" by auto2
 
@@ -125,6 +123,7 @@ theorem p39: "\<not>(\<exists>x. \<forall>y. F(y,x) \<longleftrightarrow> \<not>
   @case "F(x,x)"
 @qed
 
+(* Note there is a typo in the original text. *)
 theorem p40: "\<exists>y. \<forall>x. F(x,y) \<longleftrightarrow> F(x,x) \<Longrightarrow> \<not>(\<forall>x. \<exists>y. \<forall>z. F(z,y) \<longleftrightarrow> \<not>F(z,x))"
 @proof
   @obtain A where "\<forall>x. F(x,A) \<longleftrightarrow> F(x,x)"
