HOL/Primes_Ex.thy
@@ -1,6 +1,11 @@
 (*
   File: Primes_Ex.thy
   Author: Bohua Zhan
+
+  Elementary number theory of primes, up to the proof of infinitude
+  of primes and the unique factorization theorem.
+
+  Follows the development in HOL/Computational_Algebra/Primes.thy.
 *)
 
 section \<open>Primes\<close>
@@ -8,13 +13,6 @@ section \<open>Primes\<close>
 theory Primes_Ex
   imports Auto2_Main
 begin
-
-text \<open>
-  Elementary number theory of primes, up to the proof of infinitude
-  of primes and the unique factorization theorem.
-
-  Follows the development in HOL/Computational\_Algebra/Primes.thy.
-\<close>
 
 subsection \<open>Basic definition\<close>
 
@@ -26,7 +24,8 @@ lemma primeD2: "prime p \<Longrightarrow> m dvd p \<Longrightarrow> m = 1 \<or> 
 setup \<open>add_forward_prfstep_cond @{thm primeD2} [with_cond "?m \<noteq> 1", with_cond "?m \<noteq> ?p"]\<close>
 setup \<open>del_prfstep_thm_eqforward @{thm prime_def}\<close>
 
-lemma exists_prime [resolve]: "\<exists>p. prime p"
+(* Exists a prime p. *)
+theorem exists_prime [resolve]: "\<exists>p. prime p"
 @proof @have "prime 2" @qed
 
 lemma prime_odd_nat: "prime p \<Longrightarrow> p > 2 \<Longrightarrow> odd p" by auto2
@@ -37,7 +36,7 @@ lemma prime_dvd_mult_nat: "prime p \<Longrightarrow> p dvd m * n \<Longrightarro
 setup \<open>add_forward_prfstep_cond @{thm prime_dvd_mult_nat}
   (with_conds ["?m \<noteq> ?p", "?n \<noteq> ?p", "?m \<noteq> ?p * ?m'", "?n \<noteq> ?p * ?n'"])\<close>
 
-lemma prime_dvd_intro: "prime p \<Longrightarrow> p * q = m * n \<Longrightarrow> p dvd m \<or> p dvd n"
+theorem prime_dvd_intro: "prime p \<Longrightarrow> p * q = m * n \<Longrightarrow> p dvd m \<or> p dvd n"
 @proof @have "p dvd m * n" @qed
 setup \<open>add_forward_prfstep_cond @{thm prime_dvd_intro}
   (with_conds ["?m \<noteq> ?p", "?n \<noteq> ?p", "?m \<noteq> ?p * ?m'", "?n \<noteq> ?p * ?n'"])\<close>
@@ -90,13 +89,12 @@ lemma prime_power_mult: "prime p \<Longrightarrow> x * y = p ^ k \<Longrightarro
 
 subsection \<open>Infinitude of primes\<close>
 
-lemma bigger_prime [resolve]: "\<exists>p. prime p \<and> n < p"
+theorem bigger_prime [resolve]: "\<exists>p. prime p \<and> n < p"
 @proof
   @obtain p where "prime p" "p dvd fact n + 1"
   @case "n \<ge> p" @with @have "(p::nat) dvd fact n" @end
 @qed
 
-text \<open>Infinitude of prime numbers.\<close>
 theorem primes_infinite: "\<not> finite {p. prime p}"
 @proof
   @obtain b where "prime b" "Max {p. prime p} < b"
@@ -104,7 +102,6 @@ theorem primes_infinite: "\<not> finite {p. prime p}"
 
 subsection \<open>Existence and uniqueness of prime factorization\<close>
 
-text \<open>Existence of prime factorization.\<close>
 theorem factorization_exists: "n > 0 \<Longrightarrow> \<exists>M. (\<forall>p\<in>#M. prime p) \<and> n = (\<Prod>i\<in>#M. i)"
 @proof
   @strong_induct n
@@ -118,7 +115,7 @@ theorem factorization_exists: "n > 0 \<Longrightarrow> \<exists>M. (\<forall>p\<
   @have "n = (\<Prod>i\<in>#(M+K). i)"
 @qed
 
-lemma prime_dvd_multiset [backward1]: "prime p \<Longrightarrow> p dvd (\<Prod>i\<in>#M. i) \<Longrightarrow> \<exists>n. n\<in>#M \<and> p dvd n"
+theorem prime_dvd_multiset [backward1]: "prime p \<Longrightarrow> p dvd (\<Prod>i\<in>#M. i) \<Longrightarrow> \<exists>n. n\<in>#M \<and> p dvd n"
 @proof
   @strong_induct M
   @case "M = {#}"
@@ -126,7 +123,7 @@ lemma prime_dvd_multiset [backward1]: "prime p \<Longrightarrow> p dvd (\<Prod>i
   @contradiction @apply_induct_hyp M'
 @qed
   
-lemma factorization_unique_aux:
+theorem factorization_unique_aux:
   "\<forall>p\<in>#M. prime p \<Longrightarrow> \<forall>p\<in>#N. prime p \<Longrightarrow> (\<Prod>i\<in>#M. i) dvd (\<Prod>i\<in>#N. i) \<Longrightarrow> M \<subseteq># N"
 @proof
   @strong_induct M arbitrary N
@@ -141,7 +138,6 @@ lemma factorization_unique_aux:
 @qed
 setup \<open>add_forward_prfstep_cond @{thm factorization_unique_aux} [with_cond "?M \<noteq> ?N"]\<close>
 
-text \<open>Uniqueness of prime factorization.\<close>
 theorem factorization_unique:
   "\<forall>p\<in>#M. prime p \<Longrightarrow> \<forall>p\<in>#N. prime p \<Longrightarrow> (\<Prod>i\<in>#M. i) = (\<Prod>i\<in>#N. i) \<Longrightarrow> M = N"
 @proof @have "M \<subseteq># N" @qed
